compose/SimSymb.v
@@ -10,89 +10,157 @@ Require Import Skeleton.
 Require Import Integers.
 Require Import ASTC.
 Require Import LinkingC.
-Require SimMem.
 
 
 Set Implicit Arguments.
 
-(* I wanted to use "t" as ss0/ss_linked, but forward reference is impossible. *)
-Inductive link_exact_preserved (ss0: ident -> ident -> Prop) (sk_src: Sk.t) (sk_tgt: Sk.t) (ss_linked: ident -> ident -> Prop): Prop :=
-| link_exact_preserved_intro
-    (EXACT: forall
-        id_src id_tgt
-        (SRCIN: sk_src.(privs) id_src)
-        (TGTIN: sk_tgt.(privs) id_tgt)
-      ,
-        <<EXACT: ss0 id_src id_tgt <-> ss_linked id_src id_tgt>>)
-.
 
-(* Inductive load_exact_preserved `{SS: SimSymb.SimSymb} `{SM: SimMem.SimMem} *)
-(*           (ss0: SimSymb.t) (sk_src sk_tgt: Sk.t) *)
-(*           (sm0: SimMem.t) (skenv_src skenv_tgt: SkEnv.t): Prop := *)
-(* | exact_preserved_intro *)
-(*     (COMPAT: forall *)
-(*         id_src id_tgt b_src b_tgt *)
-(*         (SRCB: skenv_src.(Genv.find_symbol) id_src = Some b_src) *)
-(*         (TGTB: skenv_tgt.(Genv.find_symbol) id_tgt = Some b_tgt) *)
-(*       , *)
-(*         sm0.(SimMem.sim_val) (Vptr b_src Ptrofs.zero true) (Vptr b_tgt Ptrofs.zero true) <-> *)
-(*         ss0.(SimSymb.sim_symb) id_src id_tgt) *)
-(* . *)
+Module SimSymb.
 
-Class SimSymb (SM: SimMem.SimMem) :=
-{
-  t: Type;
-  sim_symb: t -> ident -> ident -> Prop;
-  wf: t -> Prop;
-  closed (ss: t) (sk_src: Sk.t) (sk_tgt: Sk.t): Prop;
-  linker :> Linker t;
-  (* link (ss0 ss1 ss_link: t): Prop; *)
-  link_spec: forall
-      ss0 sk_src0 sk_tgt0
-      ss1 sk_src1 sk_tgt1
-      (WF0: wf ss0)
-      (WF1: wf ss1)
-      (CLOSED0: closed ss0 sk_src0 sk_tgt0)
-      (CLOSED1: closed ss1 sk_src1 sk_tgt1)
-      sk_link_src sk_link_tgt
-      (LINKSRC: link sk_src0 sk_tgt0 = Some sk_link_src)
-      (LINKTGT: link sk_tgt0 sk_tgt0 = Some sk_link_tgt)
+  (* I wanted to use "t" as ss0/ss_linked, but forward reference is impossible. *)
+  Inductive link_exact_preserved (ss0: ident -> ident -> Prop) (sk_src: Sk.t) (sk_tgt: Sk.t) (ss_linked: ident -> ident -> Prop): Prop :=
+  | link_exact_preserved_intro
+      (EXACT: forall
+          id_src id_tgt
+          (SRCIN: sk_src.(privs) id_src)
+          (TGTIN: sk_tgt.(privs) id_tgt)
+        ,
+          <<EXACT: ss0 id_src id_tgt <-> ss_linked id_src id_tgt>>)
+  .
+
+  (* Inductive load_exact_preserved `{SS: SimSymb.SimSymb} `{SM: SimMem.SimMem} *)
+  (*           (ss0: SimSymb.t) (sk_src sk_tgt: Sk.t) *)
+  (*           (sm0: SimMem.t) (skenv_src skenv_tgt: SkEnv.t): Prop := *)
+  (* | exact_preserved_intro *)
+  (*     (COMPAT: forall *)
+  (*         id_src id_tgt b_src b_tgt *)
+  (*         (SRCB: skenv_src.(Genv.find_symbol) id_src = Some b_src) *)
+  (*         (TGTB: skenv_tgt.(Genv.find_symbol) id_tgt = Some b_tgt) *)
+  (*       , *)
+  (*         sm0.(SimMem.sim_val) (Vptr b_src Ptrofs.zero true) (Vptr b_tgt Ptrofs.zero true) <-> *)
+  (*         ss0.(SimSymb.sim_symb) id_src id_tgt) *)
+  (* . *)
+
+
+  Definition injective_func X Y (inj: X -> option Y): Prop := forall
+      x0 x1 y
+      (INJ0: inj x0 = Some y)
+      (INJ1: inj x1 = Some y)
     ,
-      exists ss_link, (<<WF: wf ss_link>>) /\
-                      (<<CLOSED: closed ss_link sk_link_src sk_link_tgt>>) /\
-                      (<<LINK: link ss0 ss1 = Some ss_link>>) /\
-                      (<<EXACT0: link_exact_preserved ss0.(sim_symb) sk_src0 sk_tgt0 ss_link.(sim_symb)>>) /\
-                      (<<EXACT1: link_exact_preserved ss1.(sim_symb) sk_src1 sk_tgt1 ss_link.(sim_symb)>>)
-  ;
-  load_exact_preserved: forall
-      ss sk_src sk_tgt
-      (WF: wf ss)
-      (CLOSED: closed ss sk_src sk_tgt)
-      skenv_src skenv_tgt m_src m_tgt
-      (LOADSRC: skenv_src = sk_src.(Sk.load_skenv) /\ sk_src.(Sk.load_mem) = Some m_src)
-      (LOADTGT: skenv_tgt = sk_tgt.(Sk.load_skenv) /\ sk_tgt.(Sk.load_mem) = Some m_tgt)
-    ,
-      exists sm,
-        (<<SRCM: sm.(SimMem.src_mem) = m_src>>) /\
-        (<<TGTM: sm.(SimMem.tgt_mem) = m_tgt>>) /\
-        (<<EXACT: forall
-            id_src id_tgt b_src b_tgt
-            (SRCFIND: skenv_src.(Genv.find_symbol) id_src = Some b_src)
-            (TGTFIND: skenv_tgt.(Genv.find_symbol) id_tgt = Some b_tgt)
-          ,
-            sm.(SimMem.sim_val) (Vptr b_src Ptrofs.zero true) (Vptr b_tgt Ptrofs.zero true) <->
-            ss.(sim_symb) id_src id_tgt>>)
-  ;
-}
-.
+      x0 = x1
+  .
 
-Module TMP.
-  Context `{SM: SimMem.SimMem}.
-  Context `{SS: @SimSymb SM}. (* ############## TODO 1) I declared it explicit but it requires @ 2) When I declare it implicit, it still requires @ *)
-  Axiom ss0: t.
-  Axiom i: ident.
-  Fail Check (ss0 i).
-  Coercion sim_symb: t >-> Funclass.
-  Check (ss0 i).
-End TMP.
+  (* TODO: better name *)
+  Inductive injective_rel X Y (inj: X -> Y -> Prop): Prop :=
+  | injective_domain
+      (DOMAIN: forall
+          x0 x1 y
+          (INJ0: inj x0 y)
+          (INJ1: inj x1 y)
+        ,
+          x0 = x1)
+  | injective_image
+      (IMAGE: forall
+          x y0 y1
+          (INJ0: inj x y0)
+          (INJ1: inj x y1)
+        ,
+          y0 = y1)
+  .
+
+  Inductive wf' (sim_symb: ident -> ident -> Prop) (src_ids: ident -> Prop) (tgt_ids: ident -> Prop) :=
+  | wf_intro
+      (CLOSED: forall
+          id_src id_tgt
+          (SIM: sim_symb id_src id_tgt)
+        ,
+          <<SRC: src_ids id_src>> /\ <<TGT: tgt_ids id_tgt>>)
+      (INJ: injective_rel sim_symb)
+  .
+
+  (* TODO: Try moving t into argument? sim_symb coercion gets broken and I don't know how to fix it. *)
+  Class class :=
+    {
+      t: Type;
+      src_ids: t -> ident -> Prop;
+      tgt_ids: t -> ident -> Prop;
+      sim_symb: t -> ident -> ident -> Prop;
+      wf: t -> Prop := fun ss => wf' ss.(sim_symb) ss.(src_ids) ss.(tgt_ids);
+      (* closed (ss: t) (sk_src: Sk.t) (sk_tgt: Sk.t): Prop; *)
+      linker :> Linker t;
+      (* link (ss0 ss1 ss_link: t): Prop; *)
+      (* link_spec: forall *)
+      (*     ss0 sk_src0 sk_tgt0 *)
+      (*     ss1 sk_src1 sk_tgt1 *)
+      (*     (WF0: wf ss0) *)
+      (*     (WF1: wf ss1) *)
+      (*     sk_link_src sk_link_tgt *)
+      (*     (LINKSRC: link sk_src0 sk_tgt0 = Some sk_link_src) *)
+      (*     (LINKTGT: link sk_tgt0 sk_tgt0 = Some sk_link_tgt) *)
+      (*   , *)
+      (*     exists ss_link, (<<WF: wf ss_link>>) /\ *)
+      (*                     (<<LINK: link ss0 ss1 = Some ss_link>>) /\ *)
+      (*                     (<<EXACT0: link_exact_preserved ss0.(sim_symb) sk_src0 sk_tgt0 ss_link.(sim_symb)>>) /\ *)
+      (*                     (<<EXACT1: link_exact_preserved ss1.(sim_symb) sk_src1 sk_tgt1 ss_link.(sim_symb)>>) *)
+      (* ; *)
+      sim_skenv: t -> SkEnv.t -> SkEnv.t -> Prop;
+      sim_skenv_monotone: forall
+          ss_link skenv_src skenv_tgt
+          (SIMSKENV: sim_skenv ss_link skenv_src skenv_tgt)
+          (* F_src V_src F_tgt V_tgt *)
+          (* (flesh_src: list (ident * globdef (AST.fundef F_src) V_src)) *)
+          (* (flesh_tgt: list (ident * globdef (AST.fundef F_tgt) V_tgt)) *)
+          skenv_proj_src skenv_proj_tgt
+          pubs
+          (LESRC: skenv_src.(SkEnv.project) (ss_link.(src_ids) \1/ pubs) skenv_proj_src)
+          (LETGT: skenv_tgt.(SkEnv.project) (ss_link.(tgt_ids) \1/ pubs) skenv_proj_tgt)
+          ss
+          (LE: linkorder ss ss_link)
+        ,
+          <<SIMSKENV: sim_skenv ss skenv_proj_src skenv_proj_tgt>>
+      ;
+          
+    }
+  .
+
+  Module TMP.
+    Context `{SS: class}.
+    Axiom ss0: t.
+    Axiom i: ident.
+    Fail Check (ss0 i).
+    Coercion sim_symb: t >-> Funclass.
+    Check (ss0 i).
+  End TMP.
+
+
+End SimSymb.
+
+Coercion SimSymb.sim_symb: SimSymb.t >-> Funclass.
+
+(* Module TMP. *)
+(*   Variable T: Type. *)
+(*   Context `{SS: SimSymb.class T}. *)
+(*   Axiom ss0: T. *)
+(*   Axiom i: ident. *)
+(*   Check (SimSymb.sim_symb ss0 i). *)
+(*   Fail Check (ss0 i). *)
+(*   Coercion SimSymb.sim_symb: SimSymb.class >-> Funclass. *)
+(*   Fail Check (ss0 i). *)
+(* End TMP. *)
+
+
+(* Print Coercions. *)
+
+(* Variables X: Type. *)
+(* Context `{SimSymb X}. *)
+(* Variable x: X. *)
+(* Variable i0: ident. *)
+(* Fail Check (x i0). *)
+(* Check (sim_symb x i0). *)
+(* (* Coercion sim_symb: SimSymb >-> Funclass. *) *)
+(* (* Fail Check (x i0). *) *)
+(* Coercion sim_symb: X >-> Funclass. *)
+(* Print Coercions. *)
+(* Coercion sim_symb: forall (X: Type) `{SimSymb X}, X >-> Funclass. *)
+
 
