cfrontend/CtypesC.v
@@ -1,0 +1,16 @@
+Require Import Axioms CoqlibC Maps Errors.
+Require Import AST Linking.
+Require Archi.
+
+Require Export Ctypes.
+
+Set Implicit Arguments.
+
+Definition fundef_of_fundef F (f: fundef F): AST.fundef F :=
+  match f with
+  | Internal f => AST.Internal f
+  | External ef _ _ _ => AST.External ef
+  end
+.
+
+Coercion fundef_of_fundef: fundef >-> AST.fundef.
