compose/SimSymbId.v
@@ -1,0 +1,67 @@
+Require Import Events.
+Require Import Values.
+Require Import AST.
+Require Import Asmregs.
+Require Import Memory.
+Require Import Globalenvs.
+Require Import Smallstep.
+Require Import CoqlibC.
+Require Import Skeleton.
+Require Import Integers.
+Require Import ASTC.
+Require Import LinkingC.
+Require Import SimSymb.
+Require Import MapsC.
+
+
+Set Implicit Arguments.
+
+
+(* Copied from Separation.v *)
+Inductive globalenv_preserved {F V: Type} (ge: Genv.t F V) (j: meminj) (bound: block) : Prop :=
+  | globalenv_preserved_intro
+      (DOMAIN: forall b, Plt b bound -> j b = Some(b, 0))
+      (IMAGE: forall b1 b2 delta, j b1 = Some(b2, delta) -> Plt b2 bound -> b1 = b2)
+      (SYMBOLS: forall id b, Genv.find_symbol ge id = Some b -> Plt b bound)
+      (FUNCTIONS: forall b fd, Genv.find_funct_ptr ge b = Some fd -> Plt b bound)
+      (VARINFOS: forall b gv, Genv.find_var_info ge b = Some gv -> Plt b bound)
+.
+(* This definition relies on meminj. *)
+
+Print Genv.match_genvs. (* Genv.genv_symb is very annoying *)
+
+Inductive sim_skenv (skenv0 skenv1: SkEnv.t): Prop :=
+| sim_skenv_intro
+    (NEXT: skenv0.(Genv.genv_next) = skenv1.(Genv.genv_next))
+    (* (SYMB: skenv0.(Genv.find_symbol) =1= skenv1.(Genv.find_symbol)) <--- gives bad name when "intros": x0 *)
+    (SYMB: forall id, skenv0.(Genv.find_symbol) id = skenv1.(Genv.find_symbol) id)
+    (DEFS: True) (* TODO: There are almost no info except unit. Also, flesh will overwrite these info. *)
+.
+
+Global Program Instance SymbInjId: SimSymb.class := {
+  t := unit;
+  src_ids := fun _ _ => False;
+  tgt_ids := fun _ _ => False;
+  sim_symb := fun _ _ _ => True;
+  sim_skenv (_: unit) := sim_skenv;
+}
+.
+Next Obligation.
+  inv LESRC.
+  inv LETGT.
+  inv SIMSKENV.
+  econs; eauto.
+  - eq_closure_tac.
+  - i.
+    destruct (Classical_Prop.classic (pubs id)); cycle 1.
+    + exploit NPROJ; eauto. { ii; des; eauto. } i; des.
+      exploit NPROJ0; eauto. { ii; des; eauto. } i; des.
+      eq_closure_tac. (* TODO: debug this *)
+      rewrite H0. rewrite H1. ss.
+    + exploit PROJ; eauto. i; des.
+      exploit PROJ0; eauto. i; des.
+      eq_closure_tac. (* TODO: debug this *)
+      rewrite <- H0. rewrite <- H1.
+      ss.
+Qed.
+
