compose/Skeleton.v
@@ -1,26 +1,59 @@
-Require Export AST.
+Require Import CoqlibC.
 Require Export Globalenvs.
 Require Import Memory.
+Require Import Ctypes.
+Require Export AST.
 
 Set Implicit Arguments.
 
+(* I don't want it to be "AST.program"-dependent, because of Ctypes.program *)
+(* TODO: In high level, prog_public can be dropped, as the data is already linked. Is it really so? *)
+(* Definition flesh F V := list (ident * globdef F V)%type. *)
 
 (* Skeleton Genv *)
 Module SkEnv.
 
-  Definition t := Genv.t (fundef (option signature)) unit.
+  (* TODO: Fix properly to cope with Ctypes.fundef *)
+  Definition t := Genv.t (AST.fundef (option signature)) unit.
+
+  (* Definition project F V (skenv: t) (fl: flesh F V): option (Genv.t F V). *)
+  (*   admit "". *)
+  (* Defined. *)
+
+  (* TODO: Is it OK to define it in Prop? I just need backward simulation of this. *)
+  Inductive project (skenv: t) (ids: ident -> Prop) (skenv_proj: t): Prop :=
+  | project_intro
+      (PUBLIC: skenv_proj.(Genv.genv_public) = [])
+      (* TODO: is this OK? Check if this info affects semantics except for linking *)
+      (NEXT: skenv.(Genv.genv_next) = skenv_proj.(Genv.genv_next))
+      (PROJ: forall
+          id
+          (IN: ids id)
+        ,
+          (<<SYMB: skenv.(Genv.find_symbol) id = skenv_proj.(Genv.find_symbol) id>>))
+      (* TODO: I don't need def here. IT will be overwritten. *)
+      (NPROJ: forall
+          id
+          (NIN: ~ ids id)
+        ,
+          <<NONE: skenv_proj.(Genv.find_symbol) id = None>>)
+  .
+
+  (* Definition project (skenv: t) (ids: list ident): option SkEnv.t. *)
+  (*   admit "". *)
+  (* Defined. *)
 
 End SkEnv.
 
 (* Skeleton *)
 Module Sk.
 
-  Definition t := AST.program (fundef (option signature)) unit.
+  Definition t := AST.program (AST.fundef (option signature)) unit.
 
-  Definition load_skenv: t -> SkEnv.t := @Genv.globalenv (fundef (option signature)) unit.
+  Definition load_skenv: t -> SkEnv.t := @Genv.globalenv (AST.fundef (option signature)) unit.
   (* No coercion! *)
 
-  Definition load_mem: t -> option mem := @Genv.init_mem (fundef (option signature)) unit.
+  Definition load_mem: t -> option mem := @Genv.init_mem (AST.fundef (option signature)) unit.
   (* No coercion! *)
 
 End Sk.
